ott_coq/destination_calculus_notations.v
@@ -44,7 +44,7 @@ Notation "T '↣' U" := (type_C T U) (at level 59, no associativity, U at level 
 Notation "'ᵛ-' h" := (val_H h) (at level 31, h at level 19, no associativity).
 Notation "'ᵛ+' h" := (val_D h) (at level 31, h at level 19, no associativity).
 Notation "'ᵛ()'" := (val_U).
-Notation "'λᵛ' x ⟼ t" := (val_F x t) (at level 59, x at level 19, t at level 59, right associativity).
+Notation "'λᵛ' x '⁔' m ⟼ t" := (val_F x m t) (at level 59, m at level 29, x at level 19, t at level 59, right associativity).
 Notation "'Inl' v" := (val_L v) (at level 31, right associativity, v at level 31).
 Notation "'Inr' v" := (val_R v) (at level 31, right associativity, v at level 31).
 Notation "'ᴇ' m '⁔' v" := (val_E m v) (at level 31, m at level 29, v at level 31, right associativity).
@@ -54,20 +54,20 @@ Notation "v 'ᵛ⩲' h " := (val_incr_hnames v h) (at level 30, h at level 19, n
 
 (* Terms : 40-59 *)
 Notation "t ≻ u" := (term_App t u) (at level 42, left associativity, u at next level).
-Notation "t 'ₜ;' u" := (term_PatU t u) (at level 45, left associativity, u at next level).
+Notation "t 'ᵗ;' u" := (term_PatU t u) (at level 45, left associativity, u at next level).
 Notation "t '≻case' m '{Inl' x1 ⟼ u1 , 'Inr' x2 ⟼ u2 '}'" := (term_PatS t m x1 u1 x2 u2) (at level 59, m at level 29, x1 at level 19, x2 at level 19, u1 at level 59, u2 at level 59, right associativity).
 Notation "t '≻case' m 'ᵛ(' x1 ',' x2 ')' ⟼ u" := (term_PatP t m x1 x2 u) (at level 59, m at level 29, x1 at level 19, x2 at level 19, u at level 59, right associativity).
 Notation "t '≻case' m 'ᴇ' n '⁔' x ⟼ u" := (term_PatE t m n x u) (at level 59,  m at level 29, n at level 29, x at level 19, u at level 59, right associativity).
 Notation "t '≻map' x ⟼ u" := (term_Map t x u) (at level 59, x at level 19, u at level 59, right associativity).
 Notation "'to⧔' t" := (term_ToA t) (at level 41, right associativity, t at level 41).
 Notation "'from⧔' t" := (term_FromA t) (at level 41, right associativity, t at level 41).
-Notation "'alloc' T" := (term_Alloc T) (at level 40, no associativity, T at next level).
-Notation "t ⨞ 'ᵛ()'" := (term_FillU t) (at level 43, left associativity).
-Notation "t ⨞ 'λ' x ⟼ u" := (term_FillF t x u) (at level 43, x at level 19, u at next level, left associativity).
-Notation "t ⨞ 'Inl'" := (term_FillL t) (at level 43, left associativity).
-Notation "t ⨞ 'Inr'" := (term_FillR t) (at level 43, left associativity).
-Notation "t ⨞ 'ᵛ(,)'" := (term_FillP t) (at level 43, left associativity).
-Notation "t ⨞ 'ᴇ' m" := (term_FillE t m) (at level 43, left associativity, m at level 29).
+Notation "'alloc'" := (term_Alloc).
+Notation "t '⨞()'" := (term_FillU t) (at level 43, left associativity).
+Notation "t '⨞(λ' x '⁔' m '⟼' u ')'" := (term_FillF t x m u) (at level 43, m at level 29, x at level 19, u at level 59, left associativity).
+Notation "t '⨞Inl'" := (term_FillL t) (at level 43, left associativity).
+Notation "t '⨞Inr'" := (term_FillR t) (at level 43, left associativity).
+Notation "t '⨞(,)'" := (term_FillP t) (at level 43, left associativity).
+Notation "t '⨞ᴇ' m" := (term_FillE t m) (at level 43, left associativity, m at level 29).
 Notation "t '⨞·' u" := (term_FillC t u) (at level 43, left associativity, u at next level).
 Notation "t 'ˢ[' x '≔' v ]" := (term_sub t x v) (at level 40, x at level 19, v at level 59, left associativity).
 
@@ -88,12 +88,13 @@ Notation "H 'ᵒ⟨' v1 '❟' C" := (ectx_AOpen H v1 C) (at level 66, v1 at leve
 Notation "C '∘' D" := (ectx_Comp C D) (at level 67, D at level 67, right associativity).
 Notation "C 'ᶠ[' h '≔' H '‗' v ]" := (ectx_fill C h H v) (at level 65, h at level 19, H at level 24, v at level 59, left associativity).
 
+Notation "'ᵗ' t" := (eterm_ECtxApp ectx_Id t) (at level 65, t at level 59, no associativity).
 Notation "C 'ʲ[' t ]" := (eterm_ECtxApp C t) (at level 65, t at level 59, no associativity).
 
 (* Typing and semantics : 70 - 79 *)
-Notation "G 'ᵛ⫦' v 'ː' T" := (TyR_val G v T) (at level 70, v at level 59, T at level 59, no associativity).
-Notation "G 'ᵗ⊢' j 'ː' T" := (Ty_term G j T) (at level 70, j at level 69, T at level 59, no associativity).
-Notation "G 'ᵉ⫦' C 'ː' T" := (TyR_ectx G C T) (at level 70, C at level 69, T at level 59, no associativity).
+Notation "G '⫦ᵛ' v 'ː' T" := (TyR_val G v T) (at level 70, v at level 59, T at level 59, no associativity).
+Notation "G '⊢' j 'ː' T" := (Ty_eterm G j T) (at level 70, j at level 69, T at level 59, no associativity).
+Notation "G '⫦ᵉ' C 'ː' T" := (TyR_ectx G C T) (at level 70, C at level 69, T at level 59, no associativity).
 
 Notation "j ⟶ k" := (Sem_eterm j k) (at level 70, k at level 69, no associativity).
 
